wordarray: proved corres between shallow and value for mapAccum
Proved the correspondence between the shallow and the value semantics
embedding of mapAccum. In the process, it was found that the original
shallow embedding was incorrect when an invalid range was given. Note
that some of the other proofs may be broken but this is only due to
including mapAccum in the set of abstraction functions in the value
semantics, and the other correspondences have yet to be proved.

cogent/examples/wa_connect/WordArray_Abstractions.thy
@@ -182,34 +182,8 @@ fun myslice :: "nat \<Rightarrow> nat \<Rightarrow> 'a list \<Rightarrow> 'a lis
   where
 "myslice frm to xs = List.take (to - frm) (List.drop frm xs)"
 
-(*
-lemma take_1_drop:
-  "i < length xs \<Longrightarrow> List.take (Suc 0) (List.drop i xs) = [xs ! i]"
-  apply (induct xs arbitrary: i)
-   apply (simp add: take_Suc_conv_app_nth)
-  by (simp add: drop_Suc_nth)
-
-lemma take_drop_Suc:
-  "i < l \<and> i < length xs \<Longrightarrow> 
-    List.take (l - i) (List.drop i xs) = (xs ! i) # List.take (l - Suc i) (List.drop (Suc i) xs)"
-  apply clarsimp
-  by (metis Cons_nth_drop_Suc Suc_diff_Suc take_Suc_Cons)
-*)
-
 subsection "Shallow Word Array Value Relation"
-(*
-overloading
-  valRel_word \<equiv> valRel
-begin
-definition valRel_word:
-  "\<And>\<xi> x v. valRel_word (\<xi> :: (funtyp,vabstyp) vabsfuns) (x :: ('a :: len8) word) (v :: (funtyp, vabstyp) vval) \<equiv> 
-      (if len_of TYPE('a) = 8 then v = VPrim (LU8 (ucast x))
-      else if len_of TYPE('a) = 16 then v = VPrim (LU16 (ucast x))
-      else if len_of TYPE('a) = 32 then v = VPrim (LU32 (ucast x))
-      else if len_of TYPE('a) = 64 then v = VPrim (LU64 (ucast x))
-      else False)"
-end
-*)
+
 overloading
   valRel_WordArrayUX \<equiv> valRel
 begin
@@ -226,19 +200,7 @@ begin
       else False)"
 end
 
-
-
-
-
-
-
-
-
-
-
-
-
-(*
+(* Alternate definitions for the valRel relations for word arrays
 
 
 overloading
@@ -340,7 +302,6 @@ lemma mapAccum_length:
   by (metis (no_types, lifting) Product_Type.split_def fst_conv length_append_singleton listAccumStep.simps prod.collapse)
 
 
-
 lemma 
   "map f xs = prod.fst (mapAccum (\<lambda>a b. (f a, b)) xs ())"
   by (induct xs; clarsimp split: prod.split)
@@ -372,14 +333,10 @@ definition wordarray_map_no_break':
           (\<lambda>a b. cogent_isa_pair ((WordArrayMapP.f\<^sub>f x) (ElemAO.make a b (WordArrayMapP.obsv\<^sub>f x)))) 
           (myslice (unat (WordArrayMapP.frm\<^sub>f x)) (unat (WordArrayMapP.to\<^sub>f x)) (WordArrayMapP.arr\<^sub>f x)) 
           (WordArrayMapP.acc\<^sub>f x)
-    in RR.make (xs @ ys @ zs) acc)" 
+    in (if (WordArrayMapP.frm\<^sub>f x) \<le> (WordArrayMapP.to\<^sub>f x) 
+        then RR.make (xs @ ys @ zs) acc 
+        else RR.make (WordArrayMapP.arr\<^sub>f x) acc))" 
 end
-
-
-
-
-
-
 
 context WordArray begin
 
@@ -432,9 +389,9 @@ fun \<xi>0 :: "(char list, atyp, 32 word) uabsfuns"
   where
   "\<xi>0 x y z = 
     (if x = ''wordarray_put2_0'' then upd_wa_put2_0 y z
-     else (if x = ''wordarray_get_0'' then upd_wa_get_0 y z
-           else (if x = ''wordarray_length_0'' then upd_wa_length_0 y z
-                 else False)))" 
+     else if x = ''wordarray_get_0'' then upd_wa_get_0 y z
+     else if x = ''wordarray_length_0'' then upd_wa_length_0 y z
+     else False)" 
 
 subsubsection "Value Semantics"
 
@@ -461,17 +418,17 @@ fun \<xi>m :: "(char list, vatyp) vabsfuns"
   where
   "\<xi>m x y z = 
     (if x = ''wordarray_put2_0'' then val_wa_put2 y z
-     else (if x = ''wordarray_get_0'' then val_wa_get y z
-           else (if x = ''wordarray_length_0'' then val_wa_length y z
-                 else False)))" 
+     else if x = ''wordarray_get_0'' then val_wa_get y z
+     else if x = ''wordarray_length_0'' then val_wa_length y z
+     else False)" 
 
 fun \<xi>p :: "(char list, vatyp) vabsfuns" 
   where
   "\<xi>p x y z = 
     (if x = ''wordarray_put2'' then val_wa_put2 y z
-     else (if x = ''wordarray_get'' then val_wa_get y z
-           else (if x = ''wordarray_length'' then val_wa_length y z
-                 else False)))" 
+     else if x = ''wordarray_get'' then val_wa_get y z
+     else if x = ''wordarray_length'' then val_wa_length y z
+     else False)" 
 
 subsection "Level 1 \<xi> Abstractions"
 
@@ -1133,86 +1090,12 @@ definition upd_wa_foldnb_0
         upd_wa_foldnb_bod \<xi>\<^sub>u y1 p frm to (uvalfun_to_exprfun func) acc obsv (ra \<union> rb) z))"
 
 
-
-
-\<comment>\<open> It is hard to generalise the definition for wordarray_fold because we require the type mapping
-    for functions which is only defined at compiled time, however since this doesn't change for each
-    level then it should actually be fine. However, we should change the definition to take the
-    abstract function relation as an argument so that we can generalise it. Another issue is
-    determining the read-only pointer sets. If we determine this by doing the uval_typing relation,
-    we would then need to show that 
-      \<lbrakk>uval_typing \<Xi> \<sigma> v t r w; uval_typing \<Xi> \<sigma> v t r' w'\<rbrakk> \<Longrightarrow> (r \<subseteq> r' \<or> r' \<subseteq> r)
-    or something along those lines. \<close>
-(*
-function extract_ptr :: "(char list, atyp, ptrtyp) store \<Rightarrow> (char list, atyp, ptrtyp) uval \<Rightarrow> ptrtyp set \<Rightarrow> ptrtyp set"
-  where
-"extract_ptr _ UUnit A = A" |
-"extract_ptr _ (UPrim _) A = A" |
-"extract_ptr s (UProduct a b) A = (extract_ptr s a A) \<union> (extract_ptr s b A)" |
-"extract_ptr s (USum _ a _) A = extract_ptr s a A" |
-"extract_ptr s (URecord fs) A = \<Union> (set (map ((\<lambda>a. extract_ptr s a A) \<circ> prod.fst) fs))" |
-"extract_ptr _ (UFunction _ _) A = A" | 
-"extract_ptr _ (UAFunction _ _) A = A" |
-"extract_ptr s (UAbstract a) A = 
-  (case a of (UWA (TPrim (Num t)) len arr) \<Rightarrow> A \<union> {arr + size_of_num_type t * i | i. i < len}
-      | _ \<Rightarrow> A)" |
-"extract_ptr s (UPtr p _) A = (if p \<in> A then A else 
-  (case s p of
-      option.Some a \<Rightarrow> extract_ptr s a (insert p A)
-    |  _  \<Rightarrow> insert p A))"
-  by pat_completeness auto
-term set
-termination
-  apply (relation "mlex_prod a undefined")
-  sorry
-*)
-(*
-definition upd_wa_foldnb  :: "(char list, atyp, 32 word) uabsfuns \<Rightarrow> (char list, atyp, 32 word) ufundef" 
-  where
-  "upd_wa_foldnb \<xi>\<^sub>u y z = 
-    (let (y1, y2) = y;
-         (z1, z2) = z
-      in (\<exists>p frm to acc r x t u v.
-        y2 = URecord [(UPtr p (RCon ''WordArray'' [RPrim (Num t)]), 
-                      RPtr (RCon ''WordArray'' [RPrim (Num t)])),
-                      (UPrim (LU32 frm), RPrim (Num U32)), (UPrim (LU32 to), RPrim (Num U32)),
-                      (x, RFun), (acc, upd.uval_repr acc), (UUnit, RUnit)] \<and> 
-        y1 = z1 \<and> y1 p = z1 p \<and> (\<exists>len arr. y1 p = option.Some (UAbstract (UWA (TPrim (Num U32)) len arr)) \<and> 
-          (\<forall>i<len. y1 (arr + size_of_num_type t * i) = z1 (arr + size_of_num_type t * i))) \<and> z2 = UPrim (LU32 r) \<and>
-        (case x of
-            UFunction f ts \<Rightarrow> (\<Xi>, [], [option.Some abbreviatedType1] \<turnstile> (App (Fun f ts) (Var 0)) : 
-                                TPrim (Num U32)) \<and> 
-                              upd_wa_foldnb_bod \<xi>\<^sub>u y1 p frm to (Fun f ts) acc (UUnit, {}) z
-          | UAFunction f ts \<Rightarrow> (\<Xi>, [], [option.Some abbreviatedType1] \<turnstile> (App (AFun f ts) (Var 0)) : 
-                                TPrim (Num U32)) \<and>
-                              upd_wa_foldnb_bod \<xi>\<^sub>u y1 p frm to (AFun f ts) acc (UUnit, {}) z
-          | _ \<Rightarrow> False)))"
-*)
-(*
-definition upd_wa_mapnb_0  :: "(char list, atyp, 32 word) ufundef" 
-  where
-  "upd_wa_mapnb_0 y z = 
-    (let (y1, y2) = y;
-         (z1, z2) = z 
-    in (\<exists>p frm to x.
-        y2 = URecord [(UPtr p (RCon ''WordArray'' [RPrim (Num U32)]),
-                      RPtr (RCon ''WordArray'' [RPrim (Num U32)])),
-                      (UPrim (LU32 frm), RPrim (Num U32)), (UPrim (LU32 to), RPrim (Num U32)),
-                      (x, RFun),
-                      (UUnit, RUnit), (UUnit, RUnit)] \<and>
-        y1 p = z1 p \<and> (\<exists>len arr. y1 p = option.Some (UAbstract (UWA (TPrim (Num U32)) len arr)) \<and> 
-          frame y1 ({p} \<union> {arr + 4 * i | i. i < len}) z1 ({p} \<union> {arr + 4 * i | i. i < len})) \<and>
-        (case x of
-            UFunction f ts \<Rightarrow> upd_wa_mapnb_bod_0 \<xi>0 y1 p frm to (Fun f ts) (UUnit) (UUnit, {}) z
-          | UAFunction f ts \<Rightarrow> upd_wa_mapnb_bod_0 \<xi>0 y1 p frm to (AFun f ts) (UUnit) (UUnit, {}) z
-          | _ \<Rightarrow> False)))"
-*)
 fun \<xi>1 :: "(char list, atyp, 32 word) uabsfuns" 
   where
   "\<xi>1 x y z = 
     (if x = ''wordarray_fold_no_break_0'' then upd_wa_foldnb_0 \<Xi> \<xi>0 abbreviatedType1 y z
-     else (if x = ''wordarray_map_no_break_0'' then False 
-           else \<xi>0 x y z))" 
+     else if x = ''wordarray_map_no_break_0'' then False 
+     else \<xi>0 x y z)" 
 
 subsubsection "Value Semantics"
 
@@ -1532,7 +1415,7 @@ lemma val_wa_mapAccumnb_bod_back_step:
 
 lemma val_wa_mapAccumnb_bod_preservation':
   "val_wa_mapAccumnb_bod \<xi>\<^sub>v t xs frm to f acc obsv r 
-    \<Longrightarrow> \<exists>rxs racc. r = VRecord [VAbstract(VWA t rxs), racc] \<and> length xs = length rxs"
+    \<Longrightarrow> \<exists>rxs racc. r = VRecord [VAbstract(VWA t rxs), racc] \<and> length rxs = length xs"
   apply (induct rule: val_wa_mapAccumnb_bod.induct[of _ \<xi>\<^sub>v t xs frm to f acc obsv r])
   apply (erule val_wa_mapAccumnb_bod.elims; clarsimp split: if_split_asm)
   done
@@ -1632,6 +1515,12 @@ definition val_wa_foldnbp
       x = VRecord [VAbstract (VWA t xs), VPrim (LU32 frm), VPrim (LU32 to), func, acc, obsv] \<and>
       is_vval_fun func \<and> val_wa_foldnb_bod \<xi>\<^sub>p t xs (unat frm) (unat to) (vvalfun_to_exprfun func) acc obsv y)"
 
+definition val_wa_mapAccumnbp
+  where
+  "val_wa_mapAccumnbp \<xi>\<^sub>p x y = (\<exists>t xs frm to func acc obsv. 
+      x = VRecord [VAbstract (VWA t xs), VPrim (LU32 frm), VPrim (LU32 to), func, acc, obsv] \<and>
+      is_vval_fun func \<and> val_wa_mapAccumnb_bod \<xi>\<^sub>p t xs (unat frm) (unat to) (vvalfun_to_exprfun func) acc obsv y)"
+
 fun \<xi>m1 :: "(char list, vatyp) vabsfuns" 
   where
   "\<xi>m1 x y z = 
@@ -1644,6 +1533,8 @@ fun \<xi>p1 :: "(char list, vatyp) vabsfuns"
   "\<xi>p1 x y z = 
     (if x = ''wordarray_fold_no_break'' 
       then val_wa_foldnbp \<xi>p y z
+     else if x = ''wordarray_map_no_break''
+      then val_wa_mapAccumnbp \<xi>p y z
      else \<xi>p x y z)" 
 end (* of context *)
 end
